trying heap implementation that just includes monotonic heap, and defines ref, that's it

ulib/FStar.Monotonic.Heap.fst
@@ -15,13 +15,13 @@ let emp = {
   memory    = (fun (r:nat) -> None)
 }
 
-private type ref' (a:Type0) (rel:preorder a) :Type0 = {
+private type mref' (a:Type0) (rel:preorder a) :Type0 = {
   addr: nat;
   init: a;
   mm:   bool;  //manually managed flag
 }
 
-let ref a rel = ref' a rel
+let mref a rel = mref' a rel
 
 let addr_of #a #rel r = r.addr
 
@@ -74,65 +74,65 @@ let free_mm #a #rel h r =
   { h with memory = (fun r' -> if r' = r.addr then None else h.memory r') }
 
 (*
- * update of a well-typed reference
+ * update of a well-typed mreference
  *)
 private let lemma_upd_contains_test
-  (#a:Type) (#rel:preorder a) (h0:heap) (r:ref a rel) (x:a{valid_upd h0 r x})
+  (#a:Type) (#rel:preorder a) (h0:heap) (r:mref a rel) (x:a{valid_upd h0 r x})
   :Lemma (h0 `contains` r ==>
           (let h1 = upd h0 r x in
-	   (forall (b:Type) (rel:preorder b) (r':ref b rel). (h0 `contains` r' /\ addr_of r' = addr_of r) ==> sel h1 r' == x /\
-           (forall (b:Type) (rel:preorder b) (r':ref b rel). addr_of r' <> addr_of r ==> sel h0 r' == sel h1 r')             /\
-	   (forall (b:Type) (rel:preorder b) (r':ref b rel). h0 `contains` r' <==> h1 `contains` r')                         /\
-	   (forall (b:Type) (rel:preorder b) (r':ref b rel). r' `unused_in` h0  <==> r' `unused_in` h1))))
+	   (forall (b:Type) (rel:preorder b) (r':mref b rel). (h0 `contains` r' /\ addr_of r' = addr_of r) ==> sel h1 r' == x /\
+           (forall (b:Type) (rel:preorder b) (r':mref b rel). addr_of r' <> addr_of r ==> sel h0 r' == sel h1 r')             /\
+	   (forall (b:Type) (rel:preorder b) (r':mref b rel). h0 `contains` r' <==> h1 `contains` r')                         /\
+	   (forall (b:Type) (rel:preorder b) (r':mref b rel). r' `unused_in` h0  <==> r' `unused_in` h1))))
   = ()
 
 (*
- * update of a reference that is mapped but not necessarily well-typed
+ * update of a mreference that is mapped but not necessarily well-typed
  * we cannot prove that h0 `contains` r' ==> h1 `contains` r'
- * because consider that in h0 (r:ref a) contains (| b, y:b |),
- * and that (r':ref b) s.t. r'.addr = r.addr
+ * because consider that in h0 (r:mref a) contains (| b, y:b |),
+ * and that (r':mref b) s.t. r'.addr = r.addr
  * in h0, r' is well-typed, but in h1 it's not
  *)
 private let lemma_upd_contains_not_necessarily_well_typed_test
-  (#a:Type) (#rel:preorder a) (h0:heap) (r:ref a rel) (x:a{valid_upd h0 r x})
+  (#a:Type) (#rel:preorder a) (h0:heap) (r:mref a rel) (x:a{valid_upd h0 r x})
   :Lemma ((~ (r `unused_in` h0)) ==>
           (let h1 = upd h0 r x in
 	   h1 `contains` r /\
-           (forall (b:Type) (#rel:preorder b) (r':ref b rel). addr_of r' <> addr_of r ==> sel h0 r' == sel h1 r')           /\
-	   (forall (b:Type) (#rel:preorder b) (r':ref b rel). (r'.addr <> r.addr /\ h0 `contains` r') ==> h1 `contains` r') /\
-	   (forall (b:Type) (#rel:preorder b) (r':ref b rel). r' `unused_in` h0 <==> r' `unused_in` h1)))
+           (forall (b:Type) (#rel:preorder b) (r':mref b rel). addr_of r' <> addr_of r ==> sel h0 r' == sel h1 r')           /\
+	   (forall (b:Type) (#rel:preorder b) (r':mref b rel). (r'.addr <> r.addr /\ h0 `contains` r') ==> h1 `contains` r') /\
+	   (forall (b:Type) (#rel:preorder b) (r':mref b rel). r' `unused_in` h0 <==> r' `unused_in` h1)))
   = ()
 
 (*
- * update of an unused reference
+ * update of an unused mreference
  *)
 private let lemma_upd_unused_test
-  (#a:Type) (#rel:preorder a) (h0:heap) (r:ref a rel) (x:a{valid_upd h0 r x})
+  (#a:Type) (#rel:preorder a) (h0:heap) (r:mref a rel) (x:a{valid_upd h0 r x})
   :Lemma (r `unused_in` h0 ==>
           (let h1 = upd h0 r x in
 	   h1 `contains` r /\
-           (forall (b:Type) (rel:preorder b) (r':ref b rel). addr_of r' <> addr_of r ==> sel h0 r' == sel h1 r') /\
-	   (forall (b:Type) (rel:preorder b) (r':ref b rel). h0 `contains` r' ==> h1 `contains` r')             /\
-	   (forall (b:Type) (rel:preorder b) (r':ref b rel). ~ (r' `unused_in` h0) ==> ~ (r' `unused_in` h1))))
+           (forall (b:Type) (rel:preorder b) (r':mref b rel). addr_of r' <> addr_of r ==> sel h0 r' == sel h1 r') /\
+	   (forall (b:Type) (rel:preorder b) (r':mref b rel). h0 `contains` r' ==> h1 `contains` r')             /\
+	   (forall (b:Type) (rel:preorder b) (r':mref b rel). ~ (r' `unused_in` h0) ==> ~ (r' `unused_in` h1))))
   = ()
 
 (*
- * alloc and alloc_mm behaves just like upd of an unmapped reference
+ * alloc and alloc_mm behaves just like upd of an unmapped mreference
  *)
 private let lemma_alloc_test (#a:Type) (rel:preorder a) (h0:heap) (x:a) (mm:bool)
   :Lemma (let (r, h1) = alloc rel h0 x mm in
           r `unused_in` h0 /\
 	  h1 `contains` r  /\
           is_mm r = mm     /\
-          (forall (b:Type) (rel:preorder b) (r':ref b rel). addr_of r' <> addr_of r ==> sel h0 r' == sel h1 r') /\
-          (forall (b:Type) (rel:preorder b) (r':ref b rel). h0 `contains` r' ==> h1 `contains` r')             /\
-	  (forall (b:Type) (rel:preorder b) (r':ref b rel). ~ (r' `unused_in` h0) ==> ~ (r' `unused_in` h1)))
+          (forall (b:Type) (rel:preorder b) (r':mref b rel). addr_of r' <> addr_of r ==> sel h0 r' == sel h1 r') /\
+          (forall (b:Type) (rel:preorder b) (r':mref b rel). h0 `contains` r' ==> h1 `contains` r')             /\
+	  (forall (b:Type) (rel:preorder b) (r':mref b rel). ~ (r' `unused_in` h0) ==> ~ (r' `unused_in` h1)))
   = ()
 
-private let lemma_free_mm_test (#a:Type) (rel:preorder a) (h0:heap) (r:ref a rel{h0 `contains` r /\ is_mm r})
+private let lemma_free_mm_test (#a:Type) (rel:preorder a) (h0:heap) (r:mref a rel{h0 `contains` r /\ is_mm r})
   :Lemma (let h1 = free_mm h0 r in
           r `unused_in` h1 /\
-	  (forall (b:Type) (rel:preorder b) (r':ref b rel). addr_of r' <> addr_of r ==>
+	  (forall (b:Type) (rel:preorder b) (r':mref b rel). addr_of r' <> addr_of r ==>
 	                          ((sel h0 r' == sel h1 r'                 /\
 				   (h0 `contains` r' <==> h1 `contains` r') /\
 				   (r' `unused_in` h0 <==> r' `unused_in` h1)))))
@@ -144,12 +144,9 @@ private let lemma_alloc_fresh_test (#a:Type) (rel:preorder a) (h0:heap) (x:a) (m
   = ()
 
 let lemma_contains_implies_used #a #rel h r = ()
-let lemma_contains_implies_not_weak_contains #a #rel h r = ()
-let lemma_weak_contains_implies_used #a #rel h r = ()
 let lemma_distinct_addrs_distinct_types #a #b #rel1 #rel2 h r1 r2 = ()
 let lemma_distinct_addrs_distinct_preorders #a #rel1 #rel2 h r1 r2 = ()
 let lemma_distinct_addrs_unused #a #b #rel1 #rel2 h r1 r2 = ()
-let lemma_distinct_addrs_weak_contains #a #b #rel1 #rel2 h r1 r2 = ()
 let lemma_alloc #a rel h0 x mm = ()
 let lemma_free_mm_sel #a #b #rel1 #rel2 h0 r1 r2 = ()
 let lemma_free_mm_contains #a #b #rel1 #rel2 h0 r1 r2 = ()
@@ -157,7 +154,7 @@ let lemma_free_mm_unused #a #b #rel1 #rel2 h0 r1 r2 = ()
 let lemma_sel_same_addr #a #rel h r1 r2 = ()
 let lemma_sel_upd1 #a #rel h r1 x r2 = ()
 let lemma_sel_upd2 #a #b #rel1 #rel2 h r1 r2 x = ()
-let lemma_ref_injectivity = ()
+let lemma_mref_injectivity = ()
 let lemma_in_dom_emp #a #rel r = ()
 let lemma_upd_contains #a #rel h r x = ()
 let lemma_well_typed_upd_contains #a #b #rel1 #rel2 h r1 x r2 = ()
@@ -174,4 +171,4 @@ let equal h1 h2 =
 
 let equal_extensional h1 h2 = ()
 
-let upd_upd_same_ref #a #rel h r x y = assert (equal (upd (upd h r x) r y) (upd h r y))
+let upd_upd_same_mref #a #rel h r x y = assert (equal (upd (upd h r x) r y) (upd h r y))
